
# Schema for the traditional brewing data, used to validate that the
# structure is right.

@prefix neg: <http://www.garshol.priv.no/2014/neg/> .
@prefix neu: <http://www.garshol.priv.no/2015/neu/> .
@prefix rdfs: <http://www.w3.org/2000/01/rdf-schema#> .
@prefix tbs: <http://www.garshol.priv.no/2014/trad-beer-schema/> .
@prefix tb: <http://www.garshol.priv.no/2014/trad-beer/> .
@prefix rdf: <http://www.w3.org/1999/02/22-rdf-syntax-ns#> .
@prefix dc: <http://purl.org/dc/elements/1.1/> .
@prefix geo: <http://www.w3.org/2003/01/geo/wgs84_pos#> .
@prefix luf: <http://www.garshol.priv.no/2015/luf/> .
@prefix km: <http://www.garshol.priv.no/2016/km/> .
@prefix sls: <http://www.garshol.priv.no/2015/sls/> .
@prefix voko: <http://www.garshol.priv.no/2016/voko/> .
@prefix eu: <http://www.garshol.priv.no/2017/eu/> .
@prefix dbo: <http://dbpedia.org/ontology/> .
@prefix dot: <http://www.garshol.priv.no/2016/dot/> .
@prefix xsd: <http://www.w3.org/2001/XMLSchema#> .
@prefix dbp: <http://dbpedia.org/resource/> .
@prefix sm: <http://www.garshol.priv.no/2018/sm/> .
@prefix erm: <http://www.garshol.priv.no/2019/erm/> .

# ===== META

rdfs:subClassOf rdfs:domain rdfs:Class;
  rdfs:range rdfs:Class.

# ===== TOO WIDE

geo:lat rdfs:domain rdf:Resource;
  rdfs:range xsd:decimal.

geo:long rdfs:domain rdf:Resource;
  rdfs:range xsd:decimal.

# ===== GENERAL STRUCTURAL METADATA

dc:date rdfs:domain tb:Account;
  rdfs:range rdfs:Literal;
  rdfs:comment """The date the account was either written, published, or
  received by the archive institution.""".

tb:references rdfs:domain tb:Account;
  rdfs:range rdf:Resource; # tb:Reference, really, but ...
  rdfs:comment "Lists what sources the account references.".

tb:same-informant-as rdfs:domain tb:Account;
  rdfs:range rdf:Resource; # should really be tb:Account
  rdfs:comment """Refers to another account to make it clear that both derive
  from the same informant.""".

tb:part-of rdfs:domain rdf:Resource;
  rdfs:range dbo:Place. # used to override data set inference

tb:translation rdfs:domain tb:Account;
  rdfs:range rdf:Resource;
  rdfs:comment "English translation".

# ===== FARMHOUSE DOMAIN

tb:year rdfs:domain tb:Account;
  rdfs:range xsd:decimal;
  rdfs:comment """The year the account was written, published, or received by
  the institution. Used when the exact date is unknown.""".

tb:brewer-sex rdfs:domain tb:Account;
  rdfs:range tb:Gender.

tb:malter-sex rdfs:domain tb:Account;
  rdfs:range tb:Gender;
  rdfs:comment "Who made malts? Men or women or both?".

tb:strainer rdfs:domain tb:Account;
  rdfs:range neg:Thing;
  rdfs:comment "What materials were used in the lauter tun filter.".

tb:herbs rdfs:domain tb:Account;
  rdfs:range neg:Herb;
  rdfs:comment """What herbs/spice were used in the beer. Any herb even
  mentioned is listed, even if the informant is uncertain about it.""".

tb:brewing-ended rdfs:domain tb:Account;
  rdfs:range rdfs:Literal;
  rdfs:comment "The year brewing ended in this place. Or false if still alive.".

tb:pitch-temperature rdfs:domain tb:Account;
  rdfs:range rdfs:Literal;
  rdfs:comment """Yeast pitching temperature. Give as text when precise numbers
  are not known""".

neg:informant-born rdfs:domain tb:Account;
  rdfs:range rdfs:Literal.

tb:hops rdfs:domain tb:Account;
  rdfs:range neg:Thing;
  rdfs:comment "Were the hops locally grown or bought? Needs revision.".

tb:mead rdfs:domain tb:Account;
  rdfs:range neg:Boolean;
  rdfs:comment "Did they make mead or not.".

tb:oppskake rdfs:domain tb:Account;
  rdfs:range neg:Boolean; # DEPRECRATED! will stop using
  rdfs:comment """Any kind of celebration when the beer was racked?""".

tb:oppskake2 rdfs:domain tb:Account;
  rdfs:range tb:OppskakeType;
  rdfs:comment """Were the neighbours invited to a party when the beer was
  racked? Should be redone to be more detailed.""".

tb:own-yeast rdfs:domain tb:Account;
  rdfs:range neg:Boolean;
  rdfs:comment "Did they have their own yeast.".

tb:grain rdfs:domain tb:Account;
  rdfs:range tb:GrainType;
  rdfs:comment "Main types of grain (barley, oats, ...) the malts made from.".

tb:secondary-grain rdfs:domain tb:Account;
  rdfs:range tb:GrainType;
  rdfs:comment """Less common/preferred types of grain (barley, oats, ...) the
  malts were made from.""".

neg:notes rdfs:domain tb:Account;
  rdfs:range rdfs:Literal;
  rdfs:comment "Used to keep text notes on the content.".

dc:subject rdfs:domain tb:Account;
  rdfs:range neg:Topic.

tb:own-malts rdfs:domain tb:Account;
  rdfs:range neg:Boolean;
  rdfs:comment "Did they make their own malts.".

tb:adjuncts rdfs:domain tb:Account;
  rdfs:range tb:Adjunct;
  rdfs:comment """Used for any kind of starch or sugar added to the beer besides
  the malts.""".

tb:strainer-type rdfs:domain tb:Account;
  rdfs:range tb:StrainerType;
  rdfs:comment "The most common (or oldest) type of lauter tun.".

# juniper

tb:juniper-infusion rdfs:domain tb:Account;
  rdfs:range neg:Boolean;
  rdfs:comment "Did they use juniper infusion in the beer?".

tb:juniper-preference rdfs:domain tb:Account;
  rdfs:range neg:Thing;
  rdfs:comment "What kind of juniper did they prefer?".

# terminology

tb:beer-name rdfs:domain tb:Account;
  rdfs:range rdfs:Literal;
  rdfs:comment "What did people call the good farmhouse ale?".

tb:yeast-term rdfs:domain tb:Account;
  rdfs:range rdfs:Literal.

tb:spent-grain-term rdfs:domain tb:Account;
  rdfs:range rdfs:Literal;
  rdfs:comment "The local term for the spent grain.".

# malting

tb:barley-rows rdfs:domain tb:Account;
  rdfs:range xsd:decimal;
  rdfs:comment "What type of barley was preferred for malting. Values: 2, 4, 6".

tb:malt-drying rdfs:domain tb:Account;
  rdfs:range tb:MaltDryingMethod.

tb:malt-drying-wood rdfs:domain tb:Account;
  rdfs:range neg:WoodType.

tb:shoot-length rdfs:domain tb:Account;
  rdfs:comment """Absolute length of the shoot when germination should be
  stopped, in cm.""";
  rdfs:range rdfs:Literal.

tb:shoot-length-ratio rdfs:domain tb:Account;
  rdfs:comment """The correct length of the shoot when it was time to stop
  sprouting, divided by length of the grain itself.""";
  rdfs:range rdfs:Literal.

tb:smoky rdfs:domain tb:Account;
  rdfs:comment """Whether the malts/beer should be smoky.""";
  rdfs:range neg:Boolean.

# preparations

tb:clean-with rdfs:domain tb:Account;
  rdfs:range tb:CleaningAgent;
  rdfs:comment "What was used to clean the wooden brewing vessels.".

# brewing process

tb:process rdfs:domain tb:Account;
  rdfs:range neg:Process;
  rdfs:comment "The most common (or oldest) brewing process in the area.".

neg:boiled rdfs:domain tb:Account;
  rdfs:range neg:Boolean;
  rdfs:comment """Whether the wort was boiled. When possible this should be
  indicated via tb:process. This property is for when we don't know enough to
  do that.""".

tb:juniper-boil rdfs:domain tb:Account;
  rdfs:range neg:Boolean.

neg:mash-temperature rdfs:domain tb:Account;
  rdfs:range xsd:decimal;
  rdfs:comment "Mash temperature in Celsius.".

# actually belongs on process (these are deprecated and will go away)

neg:hot-stones rdfs:domain tb:Account; # really on process
  rdfs:range neg:Boolean;
  rdfs:comment "Deprecated. Don't use.".

neg:hop-tea rdfs:domain tb:Account; # really on process
  rdfs:range neg:Boolean;
  rdfs:comment "Deprecated. Don't use.".

neg:mash-boil rdfs:domain tb:Account; # really on process
  rdfs:range neg:Boolean;
  rdfs:comment "Deprecated. Don't use.".

# time

tb:mash-boil-time rdfs:domain tb:Account;
  rdfs:comment "Mash boiling time in minutes";
  rdfs:range xsd:decimal.

tb:boil-time rdfs:domain tb:Account;
  rdfs:range rdfs:Literal;
  rdfs:comment "How long the wort was boiled, in minutes.".

tb:fermentation-time rdfs:domain tb:Account;
  rdfs:comment "Primary fermentation time, before racking, in hours";
  rdfs:range xsd:decimal;
  tbs:min 4;
  tbs:max 250.

# numerics

tb:og rdfs:domain tb:Account;
  rdfs:comment "Specific gravity of the wort before yeast is pitched";
  rdfs:range xsd:decimal;
  tbs:min 1.0;
  tbs:max 1.2.

tb:fg rdfs:domain tb:Account;
  rdfs:comment "Specific gravity of the finished beer";
  rdfs:range xsd:decimal;
  tbs:min 1.0;
  tbs:max 1.06.

tb:refracto-fg rdfs:domain tb:Account;
  rdfs:comment "Uncorrected refractometer FG";
  rdfs:range xsd:decimal;
  tbs:min 1.0;
  tbs:max 1.2.

tb:abv rdfs:domain tb:Account;
  rdfs:comment "Alcohol by volume";
  rdfs:range xsd:decimal;
  tbs:min 0.0;
  tbs:max 15.0.

tb:mash-ph rdfs:domain tb:Account;
  rdfs:range xsd:decimal;
  rdfs:comment "The pH of the mash.".

tb:malts-per-brew rdfs:domain tb:Account;
  rdfs:range xsd:decimal;
  rdfs:comment "How much malts was used per batch of beer? For the good beer.".

tb:brew-frequency rdfs:domain tb:Account;
  rdfs:range xsd:decimal;
  rdfs:comment "Number of brews per year.".

tb:brew-for rdfs:domain tb:Account;
  rdfs:range tb:Event;
  rdfs:comment "What events it was common to brew for.".

tb:batch-size rdfs:domain tb:Account;
  rdfs:range xsd:decimal;
  rdfs:comment "The normal batch size in liters, for the good beer.".

tb:small-beer-batch-size rdfs:domain tb:Account;
  rdfs:range xsd:decimal;
  rdfs:comment "The normal batch size for the small beer, in liters.".

tb:beers-pr-batch  rdfs:domain tb:Account;
  rdfs:range xsd:decimal;
  rdfs:comment """How many beers at different strengths were usually brewed
  from a single batch of malt.""".

tb:hop-wort-ratio rdfs:domain tb:Account;
  rdfs:range xsd:decimal;
  rdfs:comment "Grams of hops per liter of beer.".

tb:malt-wort-ratio rdfs:domain tb:Account;
  rdfs:range xsd:decimal.

tb:annual-malts-consumption rdfs:domain tb:Account;
  rdfs:range xsd:decimal;
  rdfs:comment "The normal household's usage of malts per year, in kilos.".

tb:annual-hops-consumption rdfs:domain tb:Account;
  rdfs:range xsd:decimal;
  rdfs:comment "The normal household's usage of hops per year, in grams.".

tb:hops-per-brew rdfs:domain tb:Account;
  rdfs:range xsd:decimal;
  rdfs:comment "Grams of hops per batch of beer. For the good beer only.".

# yeast

tb:yeast-harvest rdfs:domain tb:Account;
  rdfs:range neg:YeastHarvestPlace;
  rdfs:comment "Where was the yeast harvested from.".

tb:yeast-keeping rdfs:domain tb:Account;
  rdfs:range tb:YeastKeepingMethod;
  rdfs:comment """The most common (or oldest) method for preserving the yeast
  between brews.""".

tb:secondary-yeast-keeping rdfs:domain tb:Account;
  rdfs:range tb:YeastKeepingMethod;
  rdfs:comment """All other yeast keeping methods that are mentioned.""".

# ===== DUBIOUS

neg:mash-time rdfs:domain tb:Account;
  rdfs:comment "Mash time in minutes.";
  rdfs:range rdfs:Literal.

tb:preferred-colour rdfs:domain tb:Account;
  rdfs:range rdfs:Literal;
  rdfs:comment "What colour should the beer be?".

neg:brewing-tradition rdfs:domain tb:Account;
  rdfs:range rdfs:Literal; # FIXME: should be boolean, no?
  rdfs:comment """Did this place ever have a brewing tradition? If not
  specified we assume the value is true.""".

neg:remove-sprout rdfs:domain tb:Account;
  rdfs:range neg:Boolean;
  rdfs:comment """Whether the sprouts/rootlets were removed from the malts
  before they were used.""".

tb:grain-text rdfs:domain tb:Account;
  rdfs:range rdfs:Literal;
  rdfs:comment """The exact text in the original account describing what
  grain was malted. (Not in use.)""".

tb:juniper-berries rdfs:domain tb:Account;
  rdfs:range neg:Boolean.

tb:mash-juniper rdfs:domain tb:Account;
  rdfs:range neg:Boolean.

tb:juniper-boil-length rdfs:domain tb:Account;
  rdfs:range xsd:decimal;
  rdfs:comment "How long was the juniper infusion boiled, in minutes.".

# ===== NEG-specific

neg:fylke rdfs:domain neg:Response;
  rdfs:range dbp:Province.

neg:bygdelag rdfs:domain neg:Response;
  rdfs:range rdfs:Literal.

neg:recorded-by rdfs:domain neg:Response;
  rdfs:range rdfs:Literal.

neg:gnr rdfs:domain neg:Response;
  rdfs:range rdfs:Literal.

neg:brnr rdfs:domain neg:Response;
  rdfs:range rdfs:Literal.

tb:herbs-text rdfs:domain neg:Response;
  rdfs:range rdfs:Literal.

neg:gard rdfs:domain neg:Response;
  rdfs:range rdfs:Literal.

neg:herad rdfs:domain neg:Response;
  rdfs:range rdfs:Literal.

neg:useful rdfs:domain neg:Response;
  rdfs:range rdfs:Literal.

neg:adresse rdfs:domain neg:Response;
  rdfs:range rdfs:Literal.

neg:info-from rdfs:domain neg:Response;
  rdfs:range rdfs:Literal.

neg:summary rdfs:domain neg:Response;
  rdfs:range rdf:Resource.

# ===== NEU-specific

neu:topnr rdfs:domain tb:Account; # also on uff:Response
  rdfs:range neu:TopNummer.

neu:title rdfs:domain tb:Account; # also on uff:Response
  rdfs:range rdfs:Literal.

neu:kind rdfs:domain neu:Item;
  rdfs:range neu:ItemType.

neu:address rdfs:domain tb:Account; # also on uff:Response
  rdfs:range rdfs:Literal.

neu:informant rdfs:domain tb:Account; # also on uff:Response
  rdfs:range rdfs:Literal.

neu:response-to rdfs:domain neu:Item;
  rdfs:range rdf:Resource. # easier than tb:Reference.

neu:includes rdfs:domain neu:Item;
  rdfs:range rdfs:Literal.

# ===== LUF-specific

luf:recorded-by rdfs:domain luf:Response;
  rdfs:range rdfs:Literal.

luf:socken rdfs:domain luf:Response;
  rdfs:range rdfs:Literal.

luf:haerad rdfs:domain luf:Response;
  rdfs:range rdfs:Literal.

luf:address rdfs:domain luf:Response;
  rdfs:range rdfs:Literal.

luf:landskap rdfs:domain luf:Response;
  rdfs:range rdfs:Literal.

luf:born rdfs:domain luf:Response;
  rdfs:range rdfs:Literal.

luf:born-in rdfs:domain luf:Response;
  rdfs:range rdfs:Literal.

luf:told-by rdfs:domain luf:Response;
  rdfs:range rdfs:Literal.

luf:laen rdfs:domain luf:Response;
  rdfs:range rdfs:Literal.

# ===== KM-specific

km:informant rdfs:domain km:Account;
  rdfs:range rdfs:Literal.

km:response-to rdfs:domain km:Account;
  rdfs:range rdf:Resource. # easier than tb:Reference.

km:place rdfs:domain km:Account;
  rdfs:range rdfs:Literal.

# ===== SLS-specific

sls:informant rdfs:domain sls:Response;
  rdfs:range rdfs:Literal.

sls:born rdfs:domain sls:Response;
  rdfs:range rdfs:Literal.

sls:place rdfs:domain sls:Response;
  rdfs:range rdfs:Literal.

# ===== VOKO-specific

voko:kreis rdfs:domain voko:Manuskript;
  rdfs:range rdfs:Literal.

voko:ort rdfs:domain voko:Manuskript;
  rdfs:range rdfs:Literal.

voko:ortsteil rdfs:domain voko:Manuskript;
  rdfs:range rdfs:Literal.

voko:einsendedatum rdfs:domain voko:Manuskript;
  rdfs:range rdfs:Literal.

voko:zeitraum rdfs:domain voko:Manuskript;
  rdfs:range rdfs:Literal.

voko:zeitangabe rdfs:domain voko:Manuskript;
  rdfs:range rdfs:Literal.

voko:beschreibung rdfs:domain voko:Manuskript;
  rdfs:range rdfs:Literal.

voko:autor rdfs:domain voko:Manuskript;
  rdfs:range rdfs:Literal.

voko:title rdfs:domain voko:Manuskript;
  rdfs:range rdfs:Literal.

voko:region rdfs:domain voko:Manuskript;
  rdfs:range rdfs:Literal.

# ===== EU-specific

eu:place rdfs:domain eu:Response;
  rdfs:range rdfs:Literal.

eu:socken rdfs:domain eu:Response;
  rdfs:range rdfs:Literal.

eu:landskap rdfs:domain eu:Response;
  rdfs:range rdfs:Literal.

eu:author rdfs:domain eu:Response;
  rdfs:range rdfs:Literal.

eu:harad rdfs:domain eu:Response;
  rdfs:range rdfs:Literal.

tb:found-in rdfs:domain tb:Account;
  rdfs:range rdf:Resource; # easier than tb:Reference;
  rdfs:comment """For accounts found in published sources, refers to the
  source it was found in.""".

eu:town rdfs:domain eu:Response;
  rdfs:range rdfs:Literal.

eu:contained-in rdfs:domain eu:PseudoResponse;
  rdfs:range rdf:Resource. # easier than eu:Response.

eu:informant rdfs:domain eu:Response;
  rdfs:range rdfs:Literal.

# ===== Recipe-specific

dc:title rdfs:domain tb:Account; # also dot
  rdfs:range rdfs:Literal;
  rdfs:comment "A title for the account.".

rdfs:label rdfs:domain dbo:Place;
  rdfs:range rdfs:Literal.

tb:place-of-origin rdfs:domain tb:Account; # also dot
  rdfs:range dbo:Place;
  rdfs:comment "What place does the account describe?".

neg:year rdfs:domain tb:Recipe;
  rdfs:range rdfs:Literal;
  rdfs:comment """The year the account was written, published, or received by
  the institution. Used when the exact date (dc:date) is not known.""".

# ===== DOT-specific

# ===== SM-specific

sm:vl rdfs:domain sm:Account;
  rdfs:range rdfs:Literal.
  # not sure what it means yet

sm:aps rdfs:domain sm:Account;
  rdfs:range rdfs:Literal;
  rdfs:comment "Apskrites".

# ===== ERM-specific

erm:khk rdfs:domain erm:Account;
  rdfs:label "Kihelkond";
  rdfs:range rdfs:Literal.

erm:vld rdfs:domain erm:Account;
  rdfs:label "Vald";
  rdfs:range rdfs:Literal.

erm:kirjeldand rdfs:domain erm:Account;
  rdfs:label "Kirjeldand";
  rdfs:range rdfs:Literal.

erm:contained-in rdfs:domain erm:PseudoAccount;
  rdfs:label "Contained in";
  rdfs:range erm:Account.
